examples/sbf/verif_Ingress.v
@@ -1,0 +1,77 @@
+Require Import Coq.ZArith.BinInt.
+Require Import Coq.Program.Program.
+Require Poulet4.Utils.Utils.
+Require Import Coq.NArith.BinNat.
+Require Import Poulet4.P4light.Syntax.P4defs.
+Require Import Poulet4.P4light.Semantics.Semantics.
+Require Import ProD3.core.Core.
+Require Import ProD3.core.Tofino.
+Require Import ProD3.examples.sbf.Utils.
+Require Import ProD3.examples.sbf.common.
+Require Import ProD3.examples.sbf.P4_types.
+Require Import ProD3.examples.sbf.LightFilter.
+Require Import ProD3.examples.sbf.LightRepr.
+Require Import ProD3.examples.sbf.verif_Filter_all.
+Require Import Hammer.Plugin.Hammer.
+Import ListNotations.
+Open Scope Z_scope.
+Import ListNotations.
+
+Definition ipv4_header : Type := Z * Z.
+
+Definition is_internal (ip_addr : Z) : bool.
+Admitted.
+
+(* The bool in the return value means the packet is allowed. *)
+Definition process (f : filter) '((timestamp, ipv4) : Z * ipv4_header) : filter * option bool :=
+  if is_internal (fst ipv4) then
+    (filter_insert f (timestamp, ipv4), Some true)
+  else
+    (filter_clear f timestamp,
+      filter_query (filter_clear f timestamp) (timestamp, (snd ipv4, fst ipv4))).
+
+Definition p := ["pipe"; "ingress"].
+
+Definition ipv4_addr_w := 32%N.
+
+Definition Ingress_fd :=
+  ltac:(get_fd ["SwitchIngress"; "apply"] ge).
+
+Definition Ingress_spec : func_spec :=
+  WITH (* p *),
+    PATH p
+    MOD None [p]
+    WITH (h : ipv4_header) (tstamp : Z) (f : filter),
+      PRE
+        (ARG [update "ipv4"
+                (update "src_addr" (P4Bit ipv4_addr_w (fst h))
+                  (update "dst_addr" (P4Bit ipv4_addr_w (snd h))
+                    (force ValBaseNull (uninit_sval_of_typ None ipv4_h))))
+                (force ValBaseNull (uninit_sval_of_typ None header_t));
+              force ValBaseNull (uninit_sval_of_typ None metadata_t);
+              force ValBaseNull (uninit_sval_of_typ None ingress_intrinsic_metadata_t);
+              force ValBaseNull (uninit_sval_of_typ None ingress_intrinsic_metadata_from_parser_t);
+              force ValBaseNull (uninit_sval_of_typ None ingress_intrinsic_metadata_for_deparser_t);
+              force ValBaseNull (uninit_sval_of_typ None ingress_intrinsic_metadata_for_tm_t)
+             ]
+        (MEM []
+        (EXT [filter_repr (p ++ ["bf2_ds"]) f])))
+      POST
+        (ARG_RET [update "ipv4"
+                    (update "src_addr" (P4Bit ipv4_addr_w (fst h))
+                      (update "dst_addr" (P4Bit ipv4_addr_w (snd h))
+                        (force ValBaseNull (uninit_sval_of_typ None ipv4_h))))
+                    (force ValBaseNull (uninit_sval_of_typ None header_t));
+                  force ValBaseNull (uninit_sval_of_typ None metadata_t);
+                  update "drop_ctl" (P4Bit_option 3 (option_map Z.b2z (snd (process f (tstamp, h)))))
+                    (force ValBaseNull (uninit_sval_of_typ None ingress_intrinsic_metadata_for_deparser_t));
+                  force ValBaseNull (uninit_sval_of_typ None ingress_intrinsic_metadata_for_tm_t)
+                 ] ValBaseNull
+        (MEM []
+        (EXT [filter_repr (p ++ ["bf2_ds"]) (fst (process f (tstamp, h)))]))).
+
+Lemma Ingress_body :
+  func_sound ge Ingress_fd nil Ingress_spec.
+Proof.
+  start_function.
+Admitted.
